fsub/autosubst2_sctx/prop_typing.v
@@ -1,0 +1,35 @@
+Require Import List.
+Require Import Program.Equality.
+From Hammer Require Import Tactics.
+From Coq Require Import ssreflect ssrfun ssrbool.
+
+Require Import common.prop_as_core.
+Require Import common.prop_as_unscoped.
+Require Import fsub.autosubst2_sctx.def_as2.
+Require Import fsub.autosubst2_sctx.def_extra.
+Require Import fsub.autosubst2_sctx.prop_basic.
+Require Import fsub.autosubst2_sctx.prop_subtyping.
+
+Import SubstNotations.
+Import UnscopedNotations.
+
+Lemma typing_narrowing Γ1 Γ2 A B C t :
+  Γ2 ++ (entry_tvar A) :: Γ1 ⊢ t : C ->
+  Γ1 ⊢ B <: A ->
+  Γ2 ++ (entry_tvar B) :: Γ1 ⊢ t : C.
+Proof.
+  intro H. dependent induction H; intros; 
+    try hauto ctrs:typing.
+  - admit.
+  - apply typing_abs.
+    + eapply wf_typ_narrowing; eauto.
+    + replace (entry_var A0 :: Γ2 ++ (entry_tvar B) :: Γ1) with ((entry_var A0 :: Γ2) ++ (entry_tvar B :: Γ1)) by auto.
+      eapply IHtyping; simpl; eauto.
+  - apply typing_tabs; eauto.
+    + eapply wf_typ_narrowing; eauto.
+    + admit.
+  - eapply typing_tapp; eauto.
+    eapply subtyping_narrowing; eauto. 
+  - eapply typing_sub; eauto.
+    eapply subtyping_narrowing; eauto. 
+Admitted.
